Otway-Rees: implemented parse_msg

otway-rees/OYRS.Messages.fst
@@ -4,7 +4,7 @@ module OYRS.Messages
 module LC = LabeledCryptoAPI
 
 
-let valid_message i (m:message i) =
+let valid_message i m =
   match m with
   | Msg1 c a b ev_a -> LC.is_msg oyrs_global_usage i c public
   | Msg2 c a b ev_a ev_b -> LC.is_msg oyrs_global_usage i c public
@@ -29,3 +29,53 @@ let serialize_msg i m =
   | Msg4 c ev_a ->
     let tag = (LC.string_to_bytes #oyrs_global_usage #i "msg4") in
     LC.concat #oyrs_global_usage #i #public tag (LC.concat #oyrs_global_usage #i #public c ev_a)
+
+let parse_msg #i (sm:msg i public) =
+  LC.split #oyrs_global_usage #i #public sm `bind` (fun r1 ->
+  let (tag_bytes, rest) = r1 in
+  LC.bytes_to_string #oyrs_global_usage #i tag_bytes `bind` (fun tag ->
+  match tag with
+  | "msg1" -> (
+    LC.split #oyrs_global_usage #i #public rest `bind` (fun r2 ->
+    let (c, rest) = r2 in
+    LC.split #oyrs_global_usage #i #public rest `bind` (fun r3 ->
+    let (a_bytes, rest) = r3 in
+    LC.bytes_to_string #oyrs_global_usage #i a_bytes `bind` (fun a ->
+    LC.split #oyrs_global_usage #i #public rest `bind` (fun r4 ->
+    let (b_bytes, ev_a) = r4 in
+    LC.bytes_to_string #oyrs_global_usage #i b_bytes `bind` (fun b ->
+    Success (Msg1 c a b ev_a)
+    )))))
+  )
+  | "msg2" -> (
+    LC.split #oyrs_global_usage #i #public rest `bind` (fun r2 ->
+    let (c, rest) = r2 in
+    LC.split #oyrs_global_usage #i #public rest `bind` (fun r3 ->
+    let (a_bytes, rest) = r3 in
+    LC.bytes_to_string #oyrs_global_usage #i a_bytes `bind` (fun a ->
+    LC.split #oyrs_global_usage #i #public rest `bind` (fun r4 ->
+    let (b_bytes, rest) = r4 in
+    LC.bytes_to_string #oyrs_global_usage #i b_bytes `bind` (fun b ->
+    LC.split #oyrs_global_usage #i #public rest `bind` (fun r5 ->
+    let (ev_a, ev_b) = r5 in
+    Success (Msg2 c a b ev_a ev_b)
+    ))))))
+  )
+  | "msg3" -> (
+    LC.split #oyrs_global_usage #i #public rest `bind` (fun r2 ->
+    let (c, rest) = r2 in
+    LC.split #oyrs_global_usage #i #public rest `bind` (fun r3 ->
+    let (ev_a, ev_b) = r3 in
+    Success (Msg3 c ev_a ev_b)
+    ))
+  )
+  | "msg4" -> (
+    LC.split #oyrs_global_usage #i #public rest `bind` (fun r2 ->
+    let (c, ev_a) = r2 in
+    Success (Msg4 c ev_a)
+    )
+  )
+  | t -> Error ("incorrect tag: " ^ t)
+  ))
+
+let parse_serialize_msg_lemma i m = ()
